adding a lemma about mem

ulib/FStar.SeqProperties.fst
@@ -81,6 +81,17 @@ let rec count x s =
 val mem: 'a -> seq 'a -> Tot bool
 let mem x l = count x l > 0
 
+
+val seq_mem_k: #a:Type -> s:seq a -> n:nat{n < Seq.length s} -> 
+    Lemma (requires True)
+	  (ensures (mem (Seq.index s n) s))
+	  (decreases n)
+	  [SMTPat (mem (Seq.index s n) s)]
+let rec seq_mem_k #a s n = 
+  if n = 0 then ()
+  else let tl = tail s in
+       seq_mem_k tl (n - 1)
+
 val swap: #a:Type -> s:seq a -> i:nat{i<length s} -> j:nat{j<length s} -> Tot (seq a)
 let swap #a s i j = upd (upd s j (index s i)) i (index s j)
 
